# Variation obs en fonction du d√©placement d'une particule

$$
v(x) = \frac{(x - x_p) \wedge k }{2\pi}\Gamma_p + v_{bc}(x) \\
\frac{\partial v}{\partial x_p} = \frac{-n \wedge k}{2 \pi} \Gamma_p + v_{bc}(x)
$$

$$
\delta x_p \to \delta \omega \to \delta \psi \to \delta v \\
\omega_i(x_p) = \frac{1}{V_i} \sum_p \Gamma_p W(x_i - x_p)\\
\omega(x) = \sum_i \omega_i(x_p) W(x- x_i) \\
K \psi(x_p) = -\omega(x_p) \\
v(x_p) = R \psi(x_p)  = - RK^{-1} \omega(x_p) \\
\nabla_{x_p} v = - R K^{-1} \nabla_{x_p} \omega(x_p) \\
\nabla_{x_p} \omega_i(x_p) = \sum_p \Gamma_p \nabla_{x_p}W(x_i - x_p) \\
$$

$$
\omega_i(\theta) = \frac{1}{V_i} \sum_p \Gamma_p W(x_i - x_p - f(x_p, \theta))\\
\begin{aligned}
f(x_p, \theta) &= \sum_m v_m(x_p) \theta_m    \\
&= \sum \Phi_m(x_p) \theta_m \\
&=  NN(x_p; \theta).
\end{aligned} \\

\delta x_p \to \delta \omega \to \delta \psi \to \delta v \\
\omega(x) = \sum_p \Gamma_p W(x - x_p) \\
\Delta \psi = - \omega \\
v = \text{rot}(\psi)
$$
$$
v = \sum_m v_m  b_m \\
\partial_{b} v_i.
$$

